src/PlutusIR/Semantics/Static/Normalisation/Strong_normalisation.v
@@ -1,9 +1,0 @@
-From PlutusCert Require Import PlutusIR Type_reduction Kinding.Kinding.
-
-Inductive sn {e : ty -> ty -> Set } x : Set :=
-| SNI : (forall y, e x y -> sn y) -> sn x.
-
-Notation SN := (@sn step).
-
-Theorem strong_normalisation {Δ T K} : (Δ |-* T : K) -> SN T.
-Admitted.
