src/PlutusIR/Semantics/Static/TypeSubstitution.v
@@ -1,11 +1,13 @@
 From Equations Require Import Equations.
-From PlutusCert Require Import PlutusIR.
-From PlutusCert Require Import Analysis.FreeVars.
-Import Ty.
 
-Require Import Coq.Lists.List.
+From PlutusCert Require Import PlutusIR plutus_util util.
+
 Require Import Coq.Strings.String.
 Local Open Scope string_scope.
+Require Import Coq.Lists.List.
+Local Open Scope list_scope.
+Import ListNotations.
+
 
 (** * Regular substitution of types *)
 
@@ -25,6 +27,8 @@ Fixpoint substituteT (X : string) (U T : ty) : ty :=
     if X =? Y then Ty_Lam Y K1 T' else Ty_Lam Y K1 (substituteT X U T')
   | Ty_App T1 T2 =>
     Ty_App (substituteT X U T1) (substituteT X U T2)
+  | Ty_SOP Tss =>
+    Ty_SOP (map2 (substituteT X U) Tss)
   end.
 
 (** Multi-substitutions of types*)
@@ -38,8 +42,43 @@ Fixpoint msubstT (ss : list (string * ty)) (T : ty) : ty :=
 Require Import Lia.
 Import ListNotations.
 
-#[local]
-Definition ftv := Ty.ftv.
+(* Moved from analysis.freevars*)
+  Function ftv (T : ty) : list string :=
+    match T with
+    | Ty_Var X =>
+        [X]
+    | Ty_Fun T1 T2 =>
+        ftv T1 ++ ftv T2
+    | Ty_IFix F T =>
+        ftv F ++ ftv T
+    | Ty_Forall X K T' =>
+        remove string_dec X (ftv T')
+    | Ty_Builtin u =>
+        []
+    | Ty_Lam X K1 T' =>
+        remove string_dec X (ftv T')
+    | Ty_App T1 T2 =>
+        ftv T1 ++ ftv T2
+    | Ty_SOP Tss =>
+        flatmap2 ftv Tss
+    end.
+
+
+Fixpoint plutusTv (t : ty) : list string :=
+  match t with
+  | Ty_Var x => [x]
+  | Ty_Lam x A t => x :: (plutusTv t)
+  | Ty_Forall x A t => x :: (plutusTv t)
+  | Ty_Fun t1 t2 => plutusTv t1 ++ plutusTv t2
+  | Ty_App t1 t2 => plutusTv t1 ++ plutusTv t2
+  | Ty_IFix f1 t1 => plutusTv f1 ++ plutusTv t1
+  | Ty_Builtin d => []
+  | Ty_SOP Tss => 
+      flatmap2 plutusTv Tss
+  end.
+
+Compute (plutusTv (Ty_SOP [[Ty_Var "a"; Ty_Var "b"]; [Ty_Var "c"; Ty_Var "d"]])).
+
 
 (** Assume that we compute the substitution of U for X in (LamAbs Y K T).
     We reduce the  problem of generating a fresh type variable to generating
@@ -58,7 +97,7 @@ Definition ftv := Ty.ftv.
     formally as well.
 *)
 Definition fresh (X : string) (U T : ty) : string :=
-  "a" ++ X ++ (concat EmptyString (ftv U)) ++ (concat EmptyString (ftv T)).
+  "a" ++ X ++ (Coq.Strings.String.concat EmptyString (plutusTv U)) ++ (Coq.Strings.String.concat EmptyString (plutusTv T)).
 
 Lemma fresh__X : forall X U T,
     X <> fresh X U T.
@@ -88,17 +127,75 @@ Fixpoint size (T : ty) : nat :=
   | Ty_Builtin u => 1
   | Ty_Lam bX K T0 => 1 + size T0
   | Ty_App T1 T2 => 1 + size T1 + size T2
+  | Ty_SOP Tss => 1 + fold_right2 (fun T acc => size T + acc) 0 Tss
+  (* NOTE: Using fold_right: easier to prove with in how it "spits" out a term that is "outside of"  the recursive fold_right*)
   end.
+
+Lemma ty_sop_smaller : forall Tss Ts T,
+  In T Ts -> size T < size (Ty_SOP (Ts::Tss)).
+Proof.
+  intros. simpl. simpl.
+  induction Ts.
+  - inversion H.
+  - destruct H.
+    + subst. simpl. lia.
+    + simpl. specialize (IHTs H). lia.
+Qed.
+
+Lemma ty_sop_le2 : forall Tss T,
+  size (Ty_SOP Tss) <= size (Ty_SOP (T::Tss)).
+Proof.
+  intros. simpl. simpl.
+  induction T; simpl; auto.
+  lia.
+Qed. 
+
+
+
+Lemma size_list_smaller : forall (T : ty) (Ts : list ty) (Tss : list (list ty)),
+  In T Ts -> In Ts Tss -> size T < size (Ty_SOP Tss).
+Proof.
+  intros T Ts Tss Hin_Ts Hin_Tss. 
+  
+  induction Tss.
+  - inversion Hin_Tss.
+  - destruct Hin_Tss.
+    + subst. induction Ts.
+      * inversion Hin_Ts.
+      * apply ty_sop_smaller. auto.
+    +  specialize (IHTss H).
+      assert (size (Ty_SOP Tss) <= size (Ty_SOP (a :: Tss))).
+      { apply ty_sop_le2. }
+      lia.
+Qed.
 
 Lemma rename_preserves_size : forall T X Y,
     size T = size (rename X Y T).
 Proof.
+  intros.
   unfold rename.
-  induction T; intros; simpl; eauto.
-  - destruct (X =? t); eauto.
-  - destruct (X =? b); simpl; eauto.
-  - destruct (X =? b); simpl; eauto.
+  apply PlutusIR.ty__ind with (P := fun T => size T = size (substituteT X (Ty_Var Y) T)); intros; simpl; eauto.
+  all: try solve [destruct (X =? X0); simpl; eauto].
+  induction H; auto.
+  inversion IHForallP22.
+  induction H; auto.
+  inversion IHForallP.
+  simpl. 
+  f_equal.
+  auto.
 Qed.
+
+(* A version of map that remembers list membership. Necessary in termination argument of substituteTCA*)
+Fixpoint map' {A B : Type} (xs : list A) : (forall x : A, In x xs -> B) -> list B :=
+  match xs with
+  | [] => fun _ => []
+  | x :: xs => fun f =>
+      f x ((or_introl (eq_refl : x = x)) : In x (x::xs)) :: map' xs (fun (y : A) (Hin : In y xs) => f y (or_intror Hin : In y (x :: xs)))
+  end.
+
+
+
+(* A version of map2 that remembers list membership. Necessary in termination argument of substituteTCA*)
 
 Equations? substituteTCA (X : string) (U T : ty) : ty by wf (size T) :=
   substituteTCA X U (Ty_Var Y) =>
@@ -134,11 +231,19 @@ Equations? substituteTCA (X : string) (U T : ty) : ty by wf (size T) :=
             else
               Ty_Lam Y K (substituteTCA X U T) ;
   substituteTCA X U (Ty_App T1 T2) =>
-      Ty_App (substituteTCA X U T1) (substituteTCA X U T2)
+      Ty_App (substituteTCA X U T1) (substituteTCA X U T2);
+  substituteTCA X U (Ty_SOP Tss) => Ty_SOP (map' Tss
+         (fun (Ts : list ty) (Hin' : In Ts Tss) => 
+            map' Ts
+            (fun T Hin => substituteTCA X U T)
+          )
+         )
   .
 Proof.
   all: try solve
     [ lia
     || replace T' with (rename Y Y' T); eauto; rewrite <- rename_preserves_size; eauto
     ].
+
+    eapply size_list_smaller; eauto.
 Qed.
