src/PlutusIR/Semantics/Static/normaliser_STLC/STLC_named_typing.v
@@ -5,9 +5,7 @@ Import ListNotations.
 Local Open Scope string_scope.
 Local Open Scope list_scope.
 
-From PlutusCert Require Import PlutusIRSOP.
-
-From PlutusCert Require plutus_kinding_set.
+From PlutusCert Require PlutusIR.
 
 
 (* Example ill-kinded:
@@ -28,29 +26,29 @@ No way to unify (KB -> KB) -> K2 with KB -> KB
 (* For Uni uses our own set kinding version for plutusIR*)
 (** Kinding of types *)
 Reserved Notation "Δ '|-*' T ':' K" (at level 40, T at level 0, K at level 0).
-Inductive has_kind : list (binderTyname * kind) -> STLC_named.term -> kind -> Set :=
+Inductive has_kind : list (PlutusIR.binderTyname * PlutusIR.kind) -> STLC_named.term -> PlutusIR.kind -> Set :=
   | K_Var : forall Δ X K,
       lookup X Δ = Some K ->
       Δ |-* (tmvar X) : K
   | K_Fun : forall Δ T1 T2,
-      Δ |-* T1 : Kind_Base ->
-      Δ |-* T2 : Kind_Base ->
-      Δ |-* (@tmapp Fun T1 T2) : Kind_Base
+      Δ |-* T1 : PlutusIR.Kind_Base ->
+      Δ |-* T2 : PlutusIR.Kind_Base ->
+      Δ |-* (@tmapp Fun T1 T2) : PlutusIR.Kind_Base
   | K_IFix  : forall Δ F T K,
       Δ |-* T : K ->
-      Δ |-* F : (Kind_Arrow (Kind_Arrow K Kind_Base) (Kind_Arrow K Kind_Base)) ->
-      Δ |-* (@tmapp IFix F T) : Kind_Base
+      Δ |-* F : (PlutusIR.Kind_Arrow (PlutusIR.Kind_Arrow K PlutusIR.Kind_Base) (PlutusIR.Kind_Arrow K PlutusIR.Kind_Base)) ->
+      Δ |-* (@tmapp IFix F T) : PlutusIR.Kind_Base
   | K_Forall : forall Δ X K T,
-      ((X, K) :: Δ) |-* T : Kind_Base ->
-      Δ |-* (@tmlam ForAll X K T) : Kind_Base
+      ((X, K) :: Δ) |-* T : PlutusIR.Kind_Base ->
+      Δ |-* (@tmlam ForAll X K T) : PlutusIR.Kind_Base
   | K_Builtin : forall Δ T,
-      plutus_kinding_set.has_kind_uni T Kind_Base ->
-      Δ |-* (@tmbuiltin T) : Kind_Base (* DefaultUni built in types must be fully applied with K_DefaultUniApply *)
+      Kinding.has_kind_uni T PlutusIR.Kind_Base ->
+      Δ |-* (@tmbuiltin T) : PlutusIR.Kind_Base (* DefaultUni built in types must be fully applied with K_DefaultUniApply *)
   | K_Lam : forall Δ X K1 T K2,
       ((X, K1) :: Δ) |-* T : K2 ->
-      Δ |-* (@tmlam Lam X K1 T) : (Kind_Arrow K1 K2)
+      Δ |-* (@tmlam Lam X K1 T) : (PlutusIR.Kind_Arrow K1 K2)
   | K_App : forall Δ T1 T2 K1 K2,
-      Δ |-* T1 : (Kind_Arrow K1 K2) ->
+      Δ |-* T1 : (PlutusIR.Kind_Arrow K1 K2) ->
       Δ |-* T2 : K1 ->
       Δ |-* (@tmapp App T1 T2) : K2
 where "Δ '|-*' T ':' K" := (has_kind Δ T K).
